@prefix : <http://performedmusicontology.org/ontology/> .
@prefix owl: <http://www.w3.org/2002/07/owl#> .
@prefix rdf: <http://www.w3.org/1999/02/22-rdf-syntax-ns#> .
@prefix xml: <http://www.w3.org/XML/1998/namespace> .
@prefix xsd: <http://www.w3.org/2001/XMLSchema#> .
@prefix rdfs: <http://www.w3.org/2000/01/rdf-schema#> .
@base <http://performedmusicontology.org/ontology/> .

<http://performedmusicontology.org/ontology/> rdf:type owl:Ontology ;
                                               owl:versionIRI <http://performedmusicontology.org/ontology/> .

#################################################################
#    Annotation properties
#################################################################

###  http://metadataregistry.org/uri/profile/rdakit/toolkitDefinition
<http://metadataregistry.org/uri/profile/rdakit/toolkitDefinition> rdf:type owl:AnnotationProperty .


###  http://metadataregistry.org/uri/profile/rdakit/toolkitLabel
<http://metadataregistry.org/uri/profile/rdakit/toolkitLabel> rdf:type owl:AnnotationProperty .


###  http://metadataregistry.org/uri/profile/regap/identifier
<http://metadataregistry.org/uri/profile/regap/identifier> rdf:type owl:AnnotationProperty .


###  http://purl.org/dc/elements/1.1/title
<http://purl.org/dc/elements/1.1/title> rdf:type owl:AnnotationProperty .


###  http://www.w3.org/2004/02/skos/core#altLabel
<http://www.w3.org/2004/02/skos/core#altLabel> rdf:type owl:AnnotationProperty .


###  http://www.w3.org/2004/02/skos/core#broader
<http://www.w3.org/2004/02/skos/core#broader> rdf:type owl:AnnotationProperty .


###  http://www.w3.org/2004/02/skos/core#definition
<http://www.w3.org/2004/02/skos/core#definition> rdf:type owl:AnnotationProperty .


###  http://www.w3.org/2004/02/skos/core#inScheme
<http://www.w3.org/2004/02/skos/core#inScheme> rdf:type owl:AnnotationProperty .


###  http://www.w3.org/2004/02/skos/core#narrower
<http://www.w3.org/2004/02/skos/core#narrower> rdf:type owl:AnnotationProperty .


###  http://www.w3.org/2004/02/skos/core#prefLabel
<http://www.w3.org/2004/02/skos/core#prefLabel> rdf:type owl:AnnotationProperty .


###  http://www.w3.org/2004/02/skos/core#scopeNote
<http://www.w3.org/2004/02/skos/core#scopeNote> rdf:type owl:AnnotationProperty .


#################################################################
#    Object Properties
#################################################################

###  http://id.loc.gov/ontologies/bibframe/eventContent
<http://id.loc.gov/ontologies/bibframe/eventContent> rdf:type owl:ObjectProperty .


###  http://id.loc.gov/ontologies/bibframe/eventContentOf
<http://id.loc.gov/ontologies/bibframe/eventContentOf> rdf:type owl:ObjectProperty .


###  http://id.loc.gov/ontologies/bibframe/relatedTo
<http://id.loc.gov/ontologies/bibframe/relatedTo> rdf:type owl:ObjectProperty .


###  http://performedmusicontology.org/ontology/aggregatedIn
:aggregatedIn rdf:type owl:ObjectProperty ;
              owl:inverseOf :aggregates ;
              <http://www.w3.org/2004/02/skos/core#definition> "Property connecting an aggregated work to a work in which it is aggregated." .


###  http://performedmusicontology.org/ontology/aggregates
:aggregates rdf:type owl:ObjectProperty ;
            rdfs:subPropertyOf owl:topObjectProperty ;
            <http://www.w3.org/2004/02/skos/core#definition> "Property connecting an aggregating work to a work that it aggregates." .


###  http://performedmusicontology.org/ontology/asMemberOf
:asMemberOf rdf:type owl:ObjectProperty ;
            rdfs:comment "Use with bf:Contribution" ;
            rdfs:label "as Member of" ;
            <http://www.w3.org/2004/02/skos/core#definition> "Organization through which a person makes a contribution to a work or instance." .


###  http://performedmusicontology.org/ontology/associatedWith
:associatedWith rdf:type owl:ObjectProperty ;
                rdfs:subPropertyOf <http://id.loc.gov/ontologies/bibframe/relatedTo> ;
                rdf:type owl:SymmetricProperty ;
                rdfs:comment "Example: the Bible used at a presidential inauguration" ;
                rdfs:label "associated with" ;
                <http://www.w3.org/2004/02/skos/core#definition> "Event or Work that is associated in a general way with another event or work, instance or item." .


###  http://performedmusicontology.org/ontology/composedOf
:composedOf rdf:type owl:ObjectProperty ;
            rdfs:comment "Use with Thematic Identifer Statement, Opus Number Statement" ;
            rdfs:label "composed of" ;
            <http://www.w3.org/2004/02/skos/core#definition> "Portion of a multi-level identifier, such as a prefix or part number" .


###  http://performedmusicontology.org/ontology/createdFor
:createdFor rdf:type owl:ObjectProperty ;
            rdfs:subPropertyOf <http://id.loc.gov/ontologies/bibframe/relatedTo> ;
            rdfs:domain <http://id.loc.gov/ontologies/bibframe/Work> ;
            rdfs:range <http://id.loc.gov/ontologies/bibframe/Event> ;
            rdfs:comment "Example: a laudatory motet intended to be sung at the inauguration of a pope." ;
            rdfs:label "created for" ;
            <http://www.w3.org/2004/02/skos/core#definition> "Event for which a work is created." .


###  http://performedmusicontology.org/ontology/hasAggregatingInstance
:hasAggregatingInstance rdf:type owl:ObjectProperty ;
                        rdfs:label "aggregated in" ;
                        <http://www.w3.org/2004/02/skos/core#definition> "Property linking an aggregated work to an instance" .


###  http://performedmusicontology.org/ontology/hasDoublingMediumOfPerformance
:hasDoublingMediumOfPerformance rdf:type owl:ObjectProperty ;
                                rdfs:comment "Use with MediumPart" ;
                                rdfs:label "has Doubling Medium of Performance" ;
                                <http://www.w3.org/2004/02/skos/core#definition> "2 (or more) mediums of performance intended to be performed alternately by a single performer" .


###  http://performedmusicontology.org/ontology/hasDramaticRole
:hasDramaticRole rdf:type owl:ObjectProperty ;
                 rdfs:comment "Example: the role of Carmen in the opera Carmen." ;
                 rdfs:label "has Dramatic Role" ;
                 <http://www.w3.org/2004/02/skos/core#definition> "Property connecting a bf:Contribution to the character of a performer in a dramatic work, such as an opera, play, or film." .


###  http://performedmusicontology.org/ontology/hasEventName
:hasEventName rdf:type owl:ObjectProperty ;
              rdfs:subPropertyOf owl:topObjectProperty ;
              rdfs:domain <http://id.loc.gov/ontologies/bibframe/Event> ;
              rdfs:label "has Event Name" ;
              <http://www.w3.org/2004/02/skos/core#definition> "Name of an event, whether formal or created for metadata purposes" .


###  http://performedmusicontology.org/ontology/hasInspiration
:hasInspiration rdf:type owl:ObjectProperty ;
                rdfs:subPropertyOf <http://id.loc.gov/ontologies/bibframe/relatedTo> ;
                owl:inverseOf :inspirationFor ;
                rdfs:label "has as Inspiration" ;
                <http://www.w3.org/2004/02/skos/core#definition> "Event that inspired the creation of a work." .


###  http://performedmusicontology.org/ontology/hasKeyMode
:hasKeyMode rdf:type owl:ObjectProperty ;
            rdfs:label "has key and mode" ;
            <http://www.w3.org/2004/02/skos/core#definition> "Property linking a work to pmo:KeyMode." .


###  http://performedmusicontology.org/ontology/hasMedium
:hasMedium rdf:type owl:ObjectProperty ;
           rdfs:comment "Use with Work" ;
           rdfs:label "has Medium" ;
           <http://www.w3.org/2004/02/skos/core#definition> "Property that links a work or performance to the declared or performed medium." .


###  http://performedmusicontology.org/ontology/hasMediumOfPerformance
:hasMediumOfPerformance rdf:type owl:ObjectProperty ;
                        rdfs:comment "Examples: bass guitar; er hu; soprano; computer" ;
                        rdfs:label "has Medium Of Performance" ;
                        <http://www.w3.org/2004/02/skos/core#definition> "Specific medium of performance." .


###  http://performedmusicontology.org/ontology/hasMediumPart
:hasMediumPart rdf:type owl:ObjectProperty ;
               rdfs:range :MediumPart ;
               rdfs:label "has Medium Part" ;
               <http://www.w3.org/2004/02/skos/core#definition> "Specific element within an overall declared or performed medium, e.g., er hu, mixed chorus." .


###  http://performedmusicontology.org/ontology/hasMediumPartType
:hasMediumPartType rdf:type owl:ObjectProperty ;
                   rdfs:subPropertyOf owl:topObjectProperty ;
                   rdfs:domain :MediumPart ;
                   rdfs:range :MediumPartType ;
                   rdfs:comment "Examples: solo, ad lib, optional, offstage, amplified" ;
                   rdfs:label "has Medium Part Type" ;
                   <http://www.w3.org/2004/02/skos/core#definition> "Property that links a a pmo:MediumPart to a specific role or type of part." .


###  http://performedmusicontology.org/ontology/hasMode
:hasMode rdf:type owl:ObjectProperty ;
         rdfs:domain <http://id.loc.gov/ontologies/bibframe/Work> ;
         rdfs:range :Mode ;
         rdfs:label "has Mode" ;
         <http://www.w3.org/2004/02/skos/core#definition> "Property linking Work to Mode." .


###  http://performedmusicontology.org/ontology/hasMusicPart
:hasMusicPart rdf:type owl:ObjectProperty ;
              rdfs:comment "Use with MediumPart" ;
              rdfs:label "has Music Part" ;
              <http://www.w3.org/2004/02/skos/core#definition> "Property linking MediumPart or bf:Contribution to the specific music parts within a single medium part e.g., Violin 1, Clarinet 2." .


###  http://performedmusicontology.org/ontology/hasPerformance
:hasPerformance rdf:type owl:ObjectProperty ;
                rdfs:subPropertyOf <http://id.loc.gov/ontologies/bibframe/eventContentOf> ;
                owl:inverseOf :performanceOf ;
                rdfs:domain <http://id.loc.gov/ontologies/bibframe/Work> ;
                rdfs:range :Performance ;
                rdfs:label "has Performance" ;
                <http://www.w3.org/2004/02/skos/core#definition> "Event that is a performance of a work" .


###  http://performedmusicontology.org/ontology/hasRecording
:hasRecording rdf:type owl:ObjectProperty ;
              rdfs:subPropertyOf <http://id.loc.gov/ontologies/bibframe/eventContent> ;
              owl:inverseOf :recordingOf ;
              rdfs:domain <http://id.loc.gov/ontologies/bibframe/Event> ;
              rdfs:range <http://id.loc.gov/ontologies/bibframe/Work> ;
              rdfs:label "has Recording" ;
              <http://www.w3.org/2004/02/skos/core#definition> "Audio or video work created from the recording of event content." .


###  http://performedmusicontology.org/ontology/hasTempo
:hasTempo rdf:type owl:ObjectProperty ;
          rdfs:label "has Tempo" .


###  http://performedmusicontology.org/ontology/hasTonalCenter
:hasTonalCenter rdf:type owl:ObjectProperty ;
                rdfs:label "has Tonal Center" ;
                <http://www.w3.org/2004/02/skos/core#definition> "Property linking Work to Tonal Center" .


###  http://performedmusicontology.org/ontology/inspirationFor
:inspirationFor rdf:type owl:ObjectProperty ;
                rdfs:subPropertyOf <http://id.loc.gov/ontologies/bibframe/relatedTo> ;
                rdfs:label "Inspiration for" ;
                <http://www.w3.org/2004/02/skos/core#definition> "Work that is inspired by an event." .


###  http://performedmusicontology.org/ontology/performanceOf
:performanceOf rdf:type owl:ObjectProperty ;
               rdfs:subPropertyOf <http://id.loc.gov/ontologies/bibframe/eventContent> ;
               rdfs:domain :Performance ;
               rdfs:range <http://id.loc.gov/ontologies/bibframe/Work> ;
               rdfs:label "Performance of" ;
               <http://www.w3.org/2004/02/skos/core#definition> "Work that is realized through a performance." .


###  http://performedmusicontology.org/ontology/recordingOf
:recordingOf rdf:type owl:ObjectProperty ;
             rdfs:subPropertyOf <http://id.loc.gov/ontologies/bibframe/eventContentOf> ;
             rdfs:domain <http://id.loc.gov/ontologies/bibframe/Work> ;
             rdfs:range <http://id.loc.gov/ontologies/bibframe/Event> ;
             rdfs:label "Recording of" ;
             <http://www.w3.org/2004/02/skos/core#definition> "Event content of an audio or video work." .


#################################################################
#    Data properties
#################################################################

###  http://id.loc.gov/ontologies/bibframe/date
<http://id.loc.gov/ontologies/bibframe/date> rdf:type owl:DatatypeProperty .


###  http://performedmusicontology.org/ontology/hasDistinctPartCount
:hasDistinctPartCount rdf:type owl:DatatypeProperty ;
                      rdfs:range rdfs:Literal ;
                      rdfs:comment "Example: A work for 2 flutes has a distinct part count of 2." ;
                      rdfs:label "Number of distinct parts" ;
                      <http://www.w3.org/2004/02/skos/core#definition> "Number of distinct music parts in a performed medium, declared medium, or medium part that is not a named ensemble." .


###  http://performedmusicontology.org/ontology/hasEnsembleCount
:hasEnsembleCount rdf:type owl:DatatypeProperty ;
                  rdfs:range rdfs:Literal ;
                  rdfs:comment "Example: a work for 2 choruses and orchestra has an ensemble count of 3." ;
                  rdfs:label "Number of ensembles" ;
                  <http://www.w3.org/2004/02/skos/core#definition> "Number of named ensembles in a specified declared medium, performed medium, or medium part." .


###  http://performedmusicontology.org/ontology/hasNumberOfHands
:hasNumberOfHands rdf:type owl:DatatypeProperty ;
                  rdfs:range rdfs:Literal ;
                  rdfs:label "Number of hands" ;
                  <http://www.w3.org/2004/02/skos/core#definition> "Number of hands required for performance in works where more than one performer shares an instrument, such as piano, 4 hands, or where an atypical number of hands is specified, such as viola, 1 hand." .


###  http://performedmusicontology.org/ontology/hasOrder
:hasOrder rdf:type owl:DatatypeProperty ;
          rdfs:range rdfs:Literal ;
          rdfs:label "Order in sequence" ;
          <http://www.w3.org/2004/02/skos/core#definition> "Order an aggregated work or instance appears in an aggregating work or instance" .


###  http://performedmusicontology.org/ontology/hasPerformerCount
:hasPerformerCount rdf:type owl:DatatypeProperty ;
                   rdfs:range rdfs:Literal ;
                   rdfs:label "Number of performers" ;
                   <http://www.w3.org/2004/02/skos/core#definition> "Actual number of individual performers participating in an event or work." .


###  http://performedmusicontology.org/ontology/hasRequiredPerformerCount
:hasRequiredPerformerCount rdf:type owl:DatatypeProperty ;
                           rdfs:range rdfs:Literal ;
                           rdfs:comment "Example: A string quartet has a required performer count of 4." ;
                           rdfs:label "Required number of performers" ;
                           <http://www.w3.org/2004/02/skos/core#definition> "Minimum or suggested number of performers required to perform a declared medium." .


###  http://performedmusicontology.org/ontology/hasTrackNumber
:hasTrackNumber rdf:type owl:DatatypeProperty ;
                rdfs:range rdfs:Literal ;
                rdfs:label "Track number" ;
                <http://www.w3.org/2004/02/skos/core#definition> "Track number(s) of a compiled audio work on a sound recording." .


###  http://performedmusicontology.org/ontology/phonogramCopyrightDate
:phonogramCopyrightDate rdf:type owl:DatatypeProperty ;
                        rdfs:subPropertyOf <http://id.loc.gov/ontologies/bibframe/date> ;
                        rdfs:range xsd:dateTime ;
                        rdfs:label "Phonogram copyright date" ;
                        <http://www.w3.org/2004/02/skos/core#definition> "Phonogram copyright date for a sound recording." .


#################################################################
#    Classes
#################################################################

###  http://erlangen-crm.org/efrbroo/F31_Performance
<http://erlangen-crm.org/efrbroo/F31_Performance> rdf:type owl:Class .


###  http://id.loc.gov/ontologies/bibframe/Carrier
<http://id.loc.gov/ontologies/bibframe/Carrier> rdf:type owl:Class .


###  http://id.loc.gov/ontologies/bibframe/Contribution
<http://id.loc.gov/ontologies/bibframe/Contribution> rdf:type owl:Class .


###  http://id.loc.gov/ontologies/bibframe/EncodingFormat
<http://id.loc.gov/ontologies/bibframe/EncodingFormat> rdf:type owl:Class .


###  http://id.loc.gov/ontologies/bibframe/Event
<http://id.loc.gov/ontologies/bibframe/Event> rdf:type owl:Class .


###  http://id.loc.gov/ontologies/bibframe/Identifier
<http://id.loc.gov/ontologies/bibframe/Identifier> rdf:type owl:Class .


###  http://id.loc.gov/ontologies/bibframe/Organization
<http://id.loc.gov/ontologies/bibframe/Organization> rdf:type owl:Class .


###  http://id.loc.gov/ontologies/bibframe/PlayingSpeed
<http://id.loc.gov/ontologies/bibframe/PlayingSpeed> rdf:type owl:Class .


###  http://id.loc.gov/ontologies/bibframe/SoundCharacteristic
<http://id.loc.gov/ontologies/bibframe/SoundCharacteristic> rdf:type owl:Class .


###  http://id.loc.gov/ontologies/bibframe/TapeConfig
<http://id.loc.gov/ontologies/bibframe/TapeConfig> rdf:type owl:Class .


###  http://id.loc.gov/ontologies/bibframe/Work
<http://id.loc.gov/ontologies/bibframe/Work> rdf:type owl:Class .


###  http://performedmusicontology.org/ontology/Audition
:Audition rdf:type owl:Class ;
          rdfs:subClassOf <http://id.loc.gov/ontologies/bibframe/Event> ;
          rdfs:label "Audition" ;
          <http://www.w3.org/2004/02/skos/core#definition> "Event in which a performer or actor is applying for a position in an ensemble, cast, film, etc." .


###  http://performedmusicontology.org/ontology/BenefitConcert
:BenefitConcert rdf:type owl:Class ;
                rdfs:subClassOf :Concert ;
                <http://www.w3.org/2004/02/skos/core#definition> "Concert held for charitable purposes, i.e., to raise funds or awareness" .


###  http://performedmusicontology.org/ontology/Ceremony
:Ceremony rdf:type owl:Class ;
          rdfs:subClassOf <http://id.loc.gov/ontologies/bibframe/Event> ;
          rdfs:label "Ceremony" ;
          <http://www.w3.org/2004/02/skos/core#definition> "Ritual event, performed on special occasions (e.g., death, baptism, wedding, graduation, equinox, coronation, victory)" .


###  http://performedmusicontology.org/ontology/CommandPerformance
:CommandPerformance rdf:type owl:Class ;
                    rdfs:subClassOf :Concert ;
                    rdfs:label "Command performance" ;
                    <http://www.w3.org/2004/02/skos/core#definition> "Performance done at the request of a monarch or other head of state." .


###  http://performedmusicontology.org/ontology/Concert
:Concert rdf:type owl:Class ;
         rdfs:subClassOf <http://id.loc.gov/ontologies/bibframe/Event> ;
         rdfs:label "Concert" ;
         <http://www.w3.org/2004/02/skos/core#definition> "Live musical performance of one or more works in front of an audience" .


###  http://performedmusicontology.org/ontology/ConcertSeries
:ConcertSeries rdf:type owl:Class ;
               rdfs:subClassOf <http://id.loc.gov/ontologies/bibframe/Event> ;
               rdfs:label "Concert series" ;
               <http://www.w3.org/2004/02/skos/core#definition> "Group of concerts in the same geographic area by a single performer or brought together by a common theme, usually available for sale as a package. e.g., an orchestra concert season, a series featuring chamber ensembles." .


###  http://performedmusicontology.org/ontology/ConcertTour
:ConcertTour rdf:type owl:Class ;
             rdfs:subClassOf <http://id.loc.gov/ontologies/bibframe/Event> ;
             rdfs:label "Concert tour" ;
             <http://www.w3.org/2004/02/skos/core#definition> "Series of concerts by a performer or group of performers in different cities, countries, or locations." .


###  http://performedmusicontology.org/ontology/DeclaredMedium
:DeclaredMedium rdf:type owl:Class ;
                rdfs:label "Declared medium" ;
                <http://www.w3.org/2004/02/skos/core#definition> "Intended overall medium of performance of a musical work, as declared by the composer, a reference source, or other source." .


###  http://performedmusicontology.org/ontology/DiscCutting
:DiscCutting rdf:type owl:Class ;
             rdfs:subClassOf <http://id.loc.gov/ontologies/bibframe/SoundCharacteristic> ;
             rdfs:label "Disc cutting process" ;
             <http://www.w3.org/2004/02/skos/core#definition> "Recording process in which a stylus cuts a vertical or lateral groove into an audio disc." .


###  http://performedmusicontology.org/ontology/Discogs
:Discogs rdf:type owl:Class ;
         rdfs:subClassOf <http://id.loc.gov/ontologies/bibframe/Identifier> ;
         rdfs:label "Discogs ID" ;
         <http://www.w3.org/2004/02/skos/core#definition> "Identifier from Discogs." .


###  http://performedmusicontology.org/ontology/DramaticRole
:DramaticRole rdf:type owl:Class ;
              rdfs:comment "Example: the role of Carmen in the opera Carmen." ;
              rdfs:label "Dramatic role" ;
              <http://www.w3.org/2004/02/skos/core#definition> "Character of a performer in a dramatic work (e.g., an opera, play, video), e.g., \"Carmen\" in the opera or video \"Carmen\"." .


###  http://performedmusicontology.org/ontology/EnsembleMediumOfPerformance
:EnsembleMediumOfPerformance rdf:type owl:Class ;
                             rdfs:subClassOf :MediumOfPerformance ;
                             rdfs:comment "Examples: orchestra, jazz combo, string quartet, percussion ensemble" ;
                             rdfs:label "Ensemble type" ;
                             <http://www.w3.org/2004/02/skos/core#definition> "Named group of like or unlike mediums of performance intended to be played by multiple performers." .


###  http://performedmusicontology.org/ontology/EventName
:EventName rdf:type owl:Class ;
           rdfs:label "Event name" ;
           <http://www.w3.org/2004/02/skos/core#definition> "Name given to an event." .


###  http://performedmusicontology.org/ontology/FirstPerformance
:FirstPerformance rdf:type owl:Class ;
                  rdfs:subClassOf :Performance ;
                  rdfs:label "First performance" ;
                  <http://www.w3.org/2004/02/skos/core#definition> "The world premiere performance of a work." .


###  http://performedmusicontology.org/ontology/IndividualMediumOfPerformance
:IndividualMediumOfPerformance rdf:type owl:Class ;
                               rdfs:subClassOf :MediumOfPerformance ;
                               rdfs:comment "Examples: flute, keyboard, pi pa, typewriter" ,
                                            "Individual musical instrument, voice, or other object used as a medium of performance." ;
                               rdfs:label "Individual medium of performance" .


###  http://performedmusicontology.org/ontology/KeyMode
:KeyMode rdf:type owl:Class ;
         rdfs:comment "Examples: C major; B-flat minor" ;
         rdfs:label "Music key and mode" ;
         <http://www.w3.org/2004/02/skos/core#definition> "Key and mode of a music work when used in combination." .


###  http://performedmusicontology.org/ontology/LivePerformance
:LivePerformance rdf:type owl:Class ;
                 rdfs:subClassOf :Performance ;
                 rdfs:label "Live performance" ;
                 <http://www.w3.org/2004/02/skos/core#definition> "Performance that is recorded at a public event, rather than in a recording session." .


###  http://performedmusicontology.org/ontology/MasterClass
:MasterClass rdf:type owl:Class ;
             rdfs:subClassOf <http://id.loc.gov/ontologies/bibframe/Event> ;
             rdfs:label "Master class" ;
             <http://www.w3.org/2004/02/skos/core#definition> "Event in which a recognized performer critiques the performances of one or more other performers." .


###  http://performedmusicontology.org/ontology/MediumOfPerformance
:MediumOfPerformance rdf:type owl:Class ;
                     rdfs:label "Medium of performance" ;
                     <http://www.w3.org/2004/02/skos/core#definition> "Instruments, voices, ensembles, choruses, and other participants (actors, dancers, etc.) required for, or performing in, an event or work, including electronics, computers, installations, etc." .


###  http://performedmusicontology.org/ontology/MediumPart
:MediumPart rdf:type owl:Class ;
            rdfs:comment "Example: a string quartet has 3 medium parts: the violins; the viola; the cello" ,
                         "Use with DeclaredMedium, PerformedMedium" ;
            rdfs:label "Medium part" ;
            <http://www.w3.org/2004/02/skos/core#definition> "Medium of performance, type, etc., of a specific part of the declared or performed medium." .


###  http://performedmusicontology.org/ontology/MediumPartType
:MediumPartType rdf:type owl:Class ;
                rdfs:comment "Use with MediumPart" ;
                rdfs:label "Part type" ;
                <http://www.w3.org/2004/02/skos/core#definition> "Specific role or type of a medium part, e.g., solo, ad lib, optional, offstage, amplified" .


###  http://performedmusicontology.org/ontology/Mode
:Mode rdf:type owl:Class ;
      rdfs:comment "Examples: Dorian, Dhaivata" ;
      rdfs:label "Music mode" ;
      <http://www.w3.org/2004/02/skos/core#definition> "Musical mode of a music work." .


###  http://performedmusicontology.org/ontology/MusicBrainz
:MusicBrainz rdf:type owl:Class ;
             rdfs:subClassOf <http://id.loc.gov/ontologies/bibframe/Identifier> ;
             rdfs:label "MusicBrainz ID" ;
             <http://www.w3.org/2004/02/skos/core#definition> "Identifier from MusicBrainz" .


###  http://performedmusicontology.org/ontology/MusicPart
:MusicPart rdf:type owl:Class ;
           rdfs:comment "Use with MediumPart" ;
           rdfs:label "Music part" ;
           <http://www.w3.org/2004/02/skos/core#definition> "Specific element within an overall declared or performed medium, e.g., Violin 1, Trumpet 2." .


###  http://performedmusicontology.org/ontology/OpenMicPerformance
:OpenMicPerformance rdf:type owl:Class ;
                    rdfs:subClassOf :Performance ;
                    rdfs:label "Open mic performance" ;
                    <http://www.w3.org/2004/02/skos/core#definition> "Live performance at a coffee house, night club, or other venue by amateur performers." .


###  http://performedmusicontology.org/ontology/OpusNumber
:OpusNumber rdf:type owl:Class ;
            rdfs:subClassOf <http://id.loc.gov/ontologies/bibframe/Identifier> ;
            rdfs:comment "Example: The number 45 of Op. 45. No. 1" ;
            rdfs:label "Opus number" ;
            <http://www.w3.org/2004/02/skos/core#definition> "Primary opus number for a   musical work." .


###  http://performedmusicontology.org/ontology/OpusNumberPart
:OpusNumberPart rdf:type owl:Class ;
                rdfs:subClassOf <http://id.loc.gov/ontologies/bibframe/Identifier> ;
                rdfs:comment "Example: The number 1 of Op. 45, no. 1" ;
                rdfs:label "Opus number part" ;
                <http://www.w3.org/2004/02/skos/core#definition> "Number for a portion of an opus number." .


###  http://performedmusicontology.org/ontology/OpusNumberStatement
:OpusNumberStatement rdf:type owl:Class ;
                     rdfs:subClassOf <http://id.loc.gov/ontologies/bibframe/Identifier> ;
                     rdfs:comment "Example: Op. 45, no. 1" ;
                     rdfs:label "Opus number statement" ;
                     <http://www.w3.org/2004/02/skos/core#definition> "Statement about the opus number for a musical work." .


###  http://performedmusicontology.org/ontology/Performance
:Performance rdf:type owl:Class ;
             rdfs:subClassOf <http://erlangen-crm.org/efrbroo/F31_Performance> ,
                             <http://id.loc.gov/ontologies/bibframe/Event> ;
             rdfs:label "Performance" ;
             <http://www.w3.org/2004/02/skos/core#definition> "Event in which a performer or group of performers present a work to an audience or in a recording studio." .


###  http://performedmusicontology.org/ontology/PerformedMedium
:PerformedMedium rdf:type owl:Class ;
                 rdfs:label "Performed medium" ;
                 <http://www.w3.org/2004/02/skos/core#definition> "The overall medium of performance used in the performance of a musical work. This may or may not be the same as the declared medium of performance." .


###  http://performedmusicontology.org/ontology/RecordingSession
:RecordingSession rdf:type owl:Class ;
                  rdfs:subClassOf <http://id.loc.gov/ontologies/bibframe/Event> ;
                  rdfs:label "Recording session" ;
                  <http://www.w3.org/2004/02/skos/core#definition> "Event in which one or more performances are recorded with the aim of producing a recording for issue." .


###  http://performedmusicontology.org/ontology/Rehearsal
:Rehearsal rdf:type owl:Class ;
           rdfs:subClassOf <http://id.loc.gov/ontologies/bibframe/Event> ;
           rdfs:label "Rehearsal" ;
           <http://www.w3.org/2004/02/skos/core#definition> "Event in which a performer or group of performers prepare for a performance in a concert." .


###  http://performedmusicontology.org/ontology/RismNumber
:RismNumber rdf:type owl:Class ;
            rdfs:subClassOf <http://id.loc.gov/ontologies/bibframe/Identifier> ;
            rdfs:label "RISM number" ;
            <http://www.w3.org/2004/02/skos/core#definition> "Number from the Repertoire Internationale des Sources Musicales (RISM) online version." .


###  http://performedmusicontology.org/ontology/Tempo
:Tempo rdf:type owl:Class ;
       rdfs:label "Tempo" ;
       <http://www.w3.org/2004/02/skos/core#definition> "The speed or pace of a music work, whether declared (in a score) or performed." .


###  http://performedmusicontology.org/ontology/ThematicCatalogNumber
:ThematicCatalogNumber rdf:type owl:Class ;
                       rdfs:subClassOf <http://id.loc.gov/ontologies/bibframe/Identifier> ;
                       rdfs:comment "Example: 485 from BWV 485; 52:d1 from TWV 52:d1" ;
                       rdfs:label "Thematic catalog number" ;
                       <http://www.w3.org/2004/02/skos/core#definition> "Numeric or alphanumeric designation of a musical work as found in a thematic index for the composer (without the identifying prefix)." .


###  http://performedmusicontology.org/ontology/ThematicCatalogPrefix
:ThematicCatalogPrefix rdf:type owl:Class ;
                       rdfs:subClassOf <http://id.loc.gov/ontologies/bibframe/Identifier> ;
                       rdfs:comment "Examples: BWV from BWV 485 (Bach); M.S. from M.S. 35 (Paganini)." ;
                       rdfs:label "Thematic catalog prefix" ;
                       <http://www.w3.org/2004/02/skos/core#definition> "Prefix assigned to a thematic catalog number denoting thework from which the number originated." .


###  http://performedmusicontology.org/ontology/ThematicCatalogStatement
:ThematicCatalogStatement rdf:type owl:Class ;
                          rdfs:subClassOf <http://id.loc.gov/ontologies/bibframe/Identifier> ;
                          rdfs:comment "Example: BWV 485 (Bach); TWV 52:d1 (Telemann)" ;
                          rdfs:label "Thematic catalog number statement" ;
                          <http://www.w3.org/2004/02/skos/core#definition> "Statement about the thematic catalog number for a musical work, including both the prefix and the numeric or alphanumeric parts." .


###  http://performedmusicontology.org/ontology/TonalCenter
:TonalCenter rdf:type owl:Class ;
             rdfs:label "Tonal center" ;
             <http://www.w3.org/2004/02/skos/core#definition> "The tonal center of a music work, without mode, e.g., D, C##." .


###  http://performedmusicontology.org/ontology/VideogamePlatformIdentifier
:VideogamePlatformIdentifier rdf:type owl:Class ;
                             rdfs:subClassOf <http://id.loc.gov/ontologies/bibframe/Identifier> ;
                             rdfs:comment "Example: CUSA 54321 (a PlayStation 4 number)" ;
                             rdfs:label "Videogame platform identifier" ;
                             <http://www.w3.org/2004/02/skos/core#definition> "Identifier assigned to a video game platform." .


###  http://performedmusicontology.org/ontology/WorkComponent
:WorkComponent rdf:type owl:Class ;
               rdfs:subClassOf <http://id.loc.gov/ontologies/bibframe/Work> ;
               rdfs:comment "Examples: A rondo from a 3-movement piano concerto; Chapter 4 of a 10 chapeter book" ;
               rdfs:label "Work component" ;
               <http://www.w3.org/2004/02/skos/core#definition> "A work that is an integral part of another work, even when separated from it, e.g., a movement of a symphony, a chapter of a novel." .


###  http://www.w3.org/2004/02/skos/core#Concept
<http://www.w3.org/2004/02/skos/core#Concept> rdf:type owl:Class .


###  http://www.w3.org/2004/02/skos/core#ConceptScheme
<http://www.w3.org/2004/02/skos/core#ConceptScheme> rdf:type owl:Class .


#################################################################
#    Individuals
#################################################################

###  http://performedmusicontology.org/ontology/AAC
:AAC rdf:type owl:NamedIndividual ,
              <http://id.loc.gov/ontologies/bibframe/EncodingFormat> ;
     rdfs:label "AAC" ;
     <http://www.w3.org/2004/02/skos/core#definition> "Advanced Audio Coding format, a proprietary audio coding standard for lossy digital audio compression." .


###  http://performedmusicontology.org/ontology/AIFF
:AIFF rdf:type owl:NamedIndividual ,
               <http://id.loc.gov/ontologies/bibframe/EncodingFormat> ;
      rdfs:label "AIFF" ;
      <http://www.w3.org/2004/02/skos/core#definition> "Standard audio file format used by Apple." .


###  http://performedmusicontology.org/ontology/CdAudio
:CdAudio rdf:type owl:NamedIndividual ,
                  <http://id.loc.gov/ontologies/bibframe/Carrier> ;
         rdfs:label "CD Audio" ;
         <http://www.w3.org/2004/02/skos/core#broader> <http://rdaregistry.info/termList/RDACarrierType/1004> ;
         <http://www.w3.org/2004/02/skos/core#definition> "Optical discs that use the standard compact disc format for audio. They are 12 cm (4 3/4 in.) in diameter, and encoded as 2-channel signed 16-bit Linear PCM sampled at 44,100 Hz." .


###  http://performedmusicontology.org/ontology/DAT
:DAT rdf:type owl:NamedIndividual ,
              <http://id.loc.gov/ontologies/bibframe/Carrier> ;
     rdfs:label "DAT (Digital Audio Tape)" ;
     <http://www.w3.org/2004/02/skos/core#broader> <http://rdaregistry.info/termList/RDACarrierType/1007> ;
     <http://www.w3.org/2004/02/skos/core#definition> "Sony's proprietary Digital Audio Tape format, characterized by magnetic media enclosed in a protective shell, with the dimensions of 8 x 6 cm, 4 mm tape or 2 7/8 x 2 1/8 in., 1/8 in. tape" .


###  http://performedmusicontology.org/ontology/Disc45
:Disc45 rdf:type owl:NamedIndividual ,
                 <http://id.loc.gov/ontologies/bibframe/Carrier> ;
        rdfs:label "45 recording" ;
        <http://www.w3.org/2004/02/skos/core#broader> <http://rdaregistry.info/termList/RDACarrierType/1004> ;
        <http://www.w3.org/2004/02/skos/core#definition> "Colloquial term representing 7\" diameter vinyl audio discs with a playing speed of 45 rpm. The term does not necessarily describe the carrier accurately." .


###  http://performedmusicontology.org/ontology/Disc78
:Disc78 rdf:type owl:NamedIndividual ,
                 <http://id.loc.gov/ontologies/bibframe/Carrier> ;
        rdfs:label "78 recording" ;
        <http://www.w3.org/2004/02/skos/core#broader> <http://rdaregistry.info/termList/RDACarrierType/1004> ;
        <http://www.w3.org/2004/02/skos/core#definition> "Colloquial term representing audio discs from the 78 rpm disc era with playing speeds ranging from around 60 rpm to 130 rpm. The term does not necessarily describe the carrier accurately." .


###  http://performedmusicontology.org/ontology/DvdAudio
:DvdAudio rdf:type owl:NamedIndividual ,
                   <http://id.loc.gov/ontologies/bibframe/Carrier> ;
          rdfs:label "DVD Audio" ;
          <http://www.w3.org/2004/02/skos/core#altLabel> "DVD-A" ;
          <http://www.w3.org/2004/02/skos/core#broader> <http://rdaregistry.info/termList/RDACarrierType/1004> ;
          <http://www.w3.org/2004/02/skos/core#definition> "DVD optical discs that use the the DVD audio format. Different bit depth/sampling rate/channel combinations can be used on a single disc." .


###  http://performedmusicontology.org/ontology/DvdVideo
:DvdVideo rdf:type owl:NamedIndividual ,
                   <http://id.loc.gov/ontologies/bibframe/Carrier> ;
          rdfs:label "DVD Video" ;
          <http://www.w3.org/2004/02/skos/core#broader> <http://rdaregistry.info/termList/RDACarrierType/1060> ;
          <http://www.w3.org/2004/02/skos/core#definition> "DVD optical discs that use the DVD format to store digital video. From 2003, it has been the dominant consumer video format." .


###  http://performedmusicontology.org/ontology/EightTrack
:EightTrack rdf:type owl:NamedIndividual ,
                     <http://id.loc.gov/ontologies/bibframe/TapeConfig> ;
            rdfs:label "8-track" ;
            <http://www.w3.org/2004/02/skos/core#definition> "Magnetic tape divided into 8 audio tracks that run parallel with each other, on which sound and other electro-acoustic signals are captured." .


###  http://performedmusicontology.org/ontology/EnhancedCdAudio
:EnhancedCdAudio rdf:type owl:NamedIndividual ,
                          <http://id.loc.gov/ontologies/bibframe/Carrier> ;
                 rdfs:label "Enhanced CD Audio" ;
                 <http://www.w3.org/2004/02/skos/core#broader> <http://rdaregistry.info/termList/RDACarrierType/1004> ;
                 <http://www.w3.org/2004/02/skos/core#definition> "An optical disc containing a combination of audio and computer data for use in both CD and CD-ROM players. Usually music CDs combined with short videos or other content." .


###  http://performedmusicontology.org/ontology/EpRecord
:EpRecord rdf:type owl:NamedIndividual ,
                   <http://id.loc.gov/ontologies/bibframe/Carrier> ;
          rdfs:label "EP (Extended play)" ;
          <http://www.w3.org/2004/02/skos/core#broader> <http://rdaregistry.info/termList/RDACarrierType/1004> ;
          <http://www.w3.org/2004/02/skos/core#definition> "A music disc that contains more tracks than a single but not as many as on a typical album/LP/disc." .


###  http://performedmusicontology.org/ontology/FLAC
:FLAC rdf:type owl:NamedIndividual ,
               <http://id.loc.gov/ontologies/bibframe/EncodingFormat> ;
      rdfs:label "FLAC" ;
      <http://www.w3.org/2004/02/skos/core#definition> "Free Lossless Audio Codec, an open audio coding format for lossless compression of digital audio." .


###  http://performedmusicontology.org/ontology/FPM12
:FPM12 rdf:type owl:NamedIndividual ,
                <http://id.loc.gov/ontologies/bibframe/PlayingSpeed> ;
       rdfs:comment "Used for piano rolls" ;
       rdfs:label 120 ;
       <http://www.w3.org/2004/02/skos/core#definition> "Playing speed of 12 feet per minute x 10." .


###  http://performedmusicontology.org/ontology/FullTrack
:FullTrack rdf:type owl:NamedIndividual ,
                    <http://id.loc.gov/ontologies/bibframe/TapeConfig> ;
           rdfs:label "full track" ;
           <http://www.w3.org/2004/02/skos/core#definition> "Magnetic tape with 1 audio track on which sound and other electro-acoustic signals are captured." .


###  http://performedmusicontology.org/ontology/HalfTrack
:HalfTrack rdf:type owl:NamedIndividual ,
                    <http://id.loc.gov/ontologies/bibframe/TapeConfig> ;
           rdfs:label "half track" ;
           <http://www.w3.org/2004/02/skos/core#definition> "Magnetic tape divided into 2 audio tracks that run parallel with each other, on which sound and other electro-acoustic signals are captured." .


###  http://performedmusicontology.org/ontology/HybridSacd
:HybridSacd rdf:type owl:NamedIndividual ,
                     <http://id.loc.gov/ontologies/bibframe/Carrier> ;
            rdfs:label "Hybrid SACD" ;
            <http://www.w3.org/2004/02/skos/core#broader> <http://rdaregistry.info/termList/RDACarrierType/1004> ;
            <http://www.w3.org/2004/02/skos/core#definition> "An SACD that also is also encoded with a PCM audio layer readable by compact disc players." .


###  http://performedmusicontology.org/ontology/IPS.9
:IPS.9 rdf:type owl:NamedIndividual ,
                <http://id.loc.gov/ontologies/bibframe/PlayingSpeed> ;
       rdfs:comment "Speed occurs on half-speed mini-cassettes used in small portable recorders." ;
       rdfs:label "15/16 ips" ;
       <http://www.w3.org/2004/02/skos/core#definition> "Playing speed of 15/16 inches per second." .


###  http://performedmusicontology.org/ontology/IPS1.8
:IPS1.8 rdf:type owl:NamedIndividual ,
                 <http://id.loc.gov/ontologies/bibframe/PlayingSpeed> ;
        rdfs:comment "Speed occurs on standard audiocassettes." ;
        rdfs:label "1 7/8 ips" ;
        <http://www.w3.org/2004/02/skos/core#definition> "Playing speed of 1 7/8 inches per second." .


###  http://performedmusicontology.org/ontology/IPS15
:IPS15 rdf:type owl:NamedIndividual ,
                <http://id.loc.gov/ontologies/bibframe/PlayingSpeed> ;
       rdfs:comment "Occcurs on reel-to-reel, studio tapes." ;
       rdfs:label "15 ips" ;
       <http://www.w3.org/2004/02/skos/core#definition> "Playing speed of 15 inches per second." .


###  http://performedmusicontology.org/ontology/IPS3.75
:IPS3.75 rdf:type owl:NamedIndividual ,
                  <http://id.loc.gov/ontologies/bibframe/PlayingSpeed> ;
         rdfs:comment "Speed occurs on consumer and nonprofessional reel-to-reel tapes, cartridges and very unusual cassette tapes." ;
         rdfs:label "3.75 ips" ;
         <http://www.w3.org/2004/02/skos/core#definition> "Playing speed of 3.75 inches per second" .


###  http://performedmusicontology.org/ontology/IPS30
:IPS30 rdf:type owl:NamedIndividual ,
                <http://id.loc.gov/ontologies/bibframe/PlayingSpeed> ;
       rdfs:comment "Occurs on reel-to-reel, studio tapes, but is rarely used." ;
       rdfs:label "30 ips" ;
       <http://www.w3.org/2004/02/skos/core#definition> "Playing speed of 30 inches per second." .


###  http://performedmusicontology.org/ontology/IPS7.5
:IPS7.5 rdf:type owl:NamedIndividual ,
                 <http://id.loc.gov/ontologies/bibframe/PlayingSpeed> ;
        rdfs:comment "Speed occurs in reel-to-reel, nonprofessional, and studio tapes." ;
        rdfs:label "7.5 ips" ;
        <http://www.w3.org/2004/02/skos/core#definition> "Playing speed of 7.5 inches per second." .


###  http://performedmusicontology.org/ontology/LP
:LP rdf:type owl:NamedIndividual ,
             <http://id.loc.gov/ontologies/bibframe/Carrier> ;
    rdfs:label "LP/Vinyl" ;
    <http://www.w3.org/2004/02/skos/core#broader> <http://rdaregistry.info/termList/RDACarrierType/1004> ;
    <http://www.w3.org/2004/02/skos/core#definition> "Colloquial term representing 12\" diameter vinyl audio discs with a playing speed of 33 1/3 rpm. The term does not necessarily accurately describe the carrier." .


###  http://performedmusicontology.org/ontology/Laserdisc
:Laserdisc rdf:type owl:NamedIndividual ,
                    <http://id.loc.gov/ontologies/bibframe/Carrier> .


###  http://performedmusicontology.org/ontology/LateralCut
:LateralCut rdf:type owl:NamedIndividual ,
                     :DiscCutting ;
            rdfs:label "Lateral cut" ;
            <http://www.w3.org/2004/02/skos/core#definition> "Recording process in which a stylus cuts a side-to-side groove into a phonograph record." .


###  http://performedmusicontology.org/ontology/MP3
:MP3 rdf:type owl:NamedIndividual ,
              <http://id.loc.gov/ontologies/bibframe/EncodingFormat> ;
     rdfs:comment "MPEG Layer III Audio, and audio encoding format for digital audio." ;
     rdfs:label "MP3" .


###  http://performedmusicontology.org/ontology/MPS1.4
:MPS1.4 rdf:type owl:NamedIndividual ,
                 <http://id.loc.gov/ontologies/bibframe/PlayingSpeed> ;
        rdfs:comment "Speed is calculated from the distance the playback mechanism covers on the surface of the disc per second, and not the number of revolutions of the disc. It is associated with compact discs (CDs)" ;
        rdfs:label "1.4 mps" ;
        <http://www.w3.org/2004/02/skos/core#definition> "Playing speed of 1.4 meters per second." .


###  http://performedmusicontology.org/ontology/OrganRoll
:OrganRoll rdf:type owl:NamedIndividual ,
                    <http://id.loc.gov/ontologies/bibframe/Carrier> ;
           rdfs:label "Organ roll" ;
           <http://www.w3.org/2004/02/skos/core#broader> <http://rdaregistry.info/termList/RDACarrierType/1006> ;
           <http://www.w3.org/2004/02/skos/core#definition> "An audio roll used to operate a player piano or reproducing organ." .


###  http://performedmusicontology.org/ontology/PianoRoll
:PianoRoll rdf:type owl:NamedIndividual ,
                    <http://id.loc.gov/ontologies/bibframe/Carrier> ;
           rdfs:label "Piano roll" ;
           <http://www.w3.org/2004/02/skos/core#broader> <http://rdaregistry.info/termList/RDACarrierType/1006> ;
           <http://www.w3.org/2004/02/skos/core#definition> "Audio roll used to operate a player piano or reproducing piano." .


###  http://performedmusicontology.org/ontology/QuarterTrack
:QuarterTrack rdf:type owl:NamedIndividual ,
                       <http://id.loc.gov/ontologies/bibframe/TapeConfig> ;
              rdfs:label "quarter track" ;
              <http://www.w3.org/2004/02/skos/core#definition> "Magnetic tape divided into 4 audio tracks that run parallel with each other, in which sound and other electro-acoustic signals are captured." .


###  http://performedmusicontology.org/ontology/RPM16
:RPM16 rdf:type owl:NamedIndividual ,
                <http://id.loc.gov/ontologies/bibframe/PlayingSpeed> ;
       rdfs:comment "For audio discs" ;
       rdfs:label "16 rpm" ;
       <http://www.w3.org/2004/02/skos/core#definition> "Playing speed of 16 revolutions per minute." .


###  http://performedmusicontology.org/ontology/RPM33
:RPM33 rdf:type owl:NamedIndividual ,
                <http://id.loc.gov/ontologies/bibframe/PlayingSpeed> ;
       rdfs:comment "For audio discs." ;
       rdfs:label "33 1/3 rpm" ;
       <http://www.w3.org/2004/02/skos/core#definition> "Playing speed of 33 1/3 revolutions per minute. Often shortened to \"33\"." .


###  http://performedmusicontology.org/ontology/RPM45
:RPM45 rdf:type owl:NamedIndividual ,
                <http://id.loc.gov/ontologies/bibframe/PlayingSpeed> ;
       rdfs:comment "For audio discs." ;
       rdfs:label "45 rpm" ;
       <http://www.w3.org/2004/02/skos/core#definition> "Playing speed of 45 revolutions per minute." .


###  http://performedmusicontology.org/ontology/RPM78
:RPM78 rdf:type owl:NamedIndividual ,
                <http://id.loc.gov/ontologies/bibframe/PlayingSpeed> ;
       rdfs:comment "For audio discs" ;
       rdfs:label "78 rpm" ;
       <http://www.w3.org/2004/02/skos/core#definition> "Playing speed of 78 revolutions per minute." .


###  http://performedmusicontology.org/ontology/RPM8
:RPM8 rdf:type owl:NamedIndividual ,
               <http://id.loc.gov/ontologies/bibframe/PlayingSpeed> ;
      rdfs:comment "For audio discs" ;
      rdfs:label "8 rpm" ;
      <http://www.w3.org/2004/02/skos/core#definition> "Playing speed of 8 revolutions per minute." .


###  http://performedmusicontology.org/ontology/Sacd
:Sacd rdf:type owl:NamedIndividual ,
               <http://id.loc.gov/ontologies/bibframe/Carrier> ;
      rdfs:label "SACD" ;
      <http://www.w3.org/2004/02/skos/core#altLabel> "Super audio compact disc" ;
      <http://www.w3.org/2004/02/skos/core#broader> <http://rdaregistry.info/termList/RDACarrierType/1004> ;
      <http://www.w3.org/2004/02/skos/core#definition> "Optical audio disc with more channels and longer playing time than a conventional CD." .


###  http://performedmusicontology.org/ontology/SixteenTrack
:SixteenTrack rdf:type owl:NamedIndividual ,
                       <http://id.loc.gov/ontologies/bibframe/TapeConfig> ;
              rdfs:label "16-track" ;
              <http://www.w3.org/2004/02/skos/core#definition> "Magnetic tape divided into 16 audio tracks that run parallel with each other, on which sound and other electro-acoustic signals are captured." .


###  http://performedmusicontology.org/ontology/TwelveTrack
:TwelveTrack rdf:type owl:NamedIndividual ,
                      <http://id.loc.gov/ontologies/bibframe/TapeConfig> ;
             rdfs:label "12-track" ;
             <http://www.w3.org/2004/02/skos/core#definition> "Magnetic tape divided into 12 audio tracks that run parallel with each other, on which sound and other electro-acoustic signals are captured." .


###  http://performedmusicontology.org/ontology/Vertical
:Vertical rdf:type owl:NamedIndividual ,
                   :DiscCutting ;
          rdfs:label "Vertical cut" ;
          <http://www.w3.org/2004/02/skos/core#altLabel> "Hill and dale" ;
          <http://www.w3.org/2004/02/skos/core#definition> "Recording process in which a stylus cuts a vertical groove into a phonograph record." .


###  http://performedmusicontology.org/ontology/adLib
:adLib rdf:type owl:NamedIndividual ,
                :MediumPartType ;
       rdfs:label "ad lib" ;
       <http://www.w3.org/2004/02/skos/core#altLabel> "ad libitum" ;
       <http://www.w3.org/2004/02/skos/core#definition> "Mediums of performance marked \"ad lib\" or \"ad libitum\" in a score or otherwise." .


###  http://performedmusicontology.org/ontology/amplified
:amplified rdf:type owl:NamedIndividual ,
                    :MediumPartType ;
           rdfs:comment "For mediums of performance marked \"amplified\" in a score or otherwise." .


###  http://performedmusicontology.org/ontology/obligato
:obligato rdf:type owl:NamedIndividual ,
                   :MediumPartType ;
          rdfs:label "obligato" ;
          <http://www.w3.org/2004/02/skos/core#definition> "For mediums of performance marked \"obligato\" in a score or otherwise." .


###  http://performedmusicontology.org/ontology/offstage
:offstage rdf:type owl:NamedIndividual ,
                   :MediumPartType ;
          rdfs:label "offstage" ;
          <http://www.w3.org/2004/02/skos/core#definition> "Declared or performed medium that is to be performed or is performed offstage, i.e., out of sight of the audience." .


###  http://performedmusicontology.org/ontology/optional
:optional rdf:type owl:NamedIndividual ,
                   :MediumPartType ;
          rdfs:label "optional" ;
          <http://www.w3.org/2004/02/skos/core#definition> "Mediums of performance marked \"optional\" in a score or otherwise." .


###  http://performedmusicontology.org/ontology/solo
:solo rdf:type owl:NamedIndividual ,
               :MediumPartType ;
      rdfs:comment "Examples: the oboe part in an oboe concerto; the soprano in a work for soprano and orchestra" ;
      rdfs:label "solo" ;
      <http://www.w3.org/2004/02/skos/core#definition> "Mediums of performance marked \"solo\" in a score or is clearly a solo part in the context of the work, e.g., a concerto for oboe and orchestra." .


###  http://rdaregistry.info/termList/RDACarrierType
<http://rdaregistry.info/termList/RDACarrierType> rdf:type owl:NamedIndividual ,
                                                           <http://www.w3.org/2004/02/skos/core#ConceptScheme> ;
                                                  <http://purl.org/dc/elements/1.1/title> "RDA Carrier Type" .


###  http://rdaregistry.info/termList/RDACarrierType/1003
<http://rdaregistry.info/termList/RDACarrierType/1003> rdf:type owl:NamedIndividual ,
                                                                <http://www.w3.org/2004/02/skos/core#Concept> ;
                                                       <http://metadataregistry.org/uri/profile/rdakit/toolkitDefinition> "A carrier type consisting of a roller-shaped object on which sound waves are incised or indented in a continuous circular groove."@en ,
                                                                                                                          "Bærertype, der består af et rulleformet genstand, hvorpå lydbølger er indskåret eller indtrykt i en uafbrudt cirkulær rille."@da ,
                                                                                                                          "Een rolvormig object waarop geluidsgolven worden ingesneden of ingesprongen in een continue cirkelvormige groef."@nl ,
                                                                                                                          "Ein Datenträgertyp, der aus einem rollenförmigen Objekt besteht, auf dem Schallwellen in einer fortlaufend gewundenen Rille graviert oder eingeprägt sind."@de ,
                                                                                                                          "En bærertype som består av en sylinderformet gjenstand der lydopptak er gravert inn i et uavbrutt, sirkulært spor."@no ,
                                                                                                                          "Loại hộp chứa gồm có vật thể hình trục lăn trên đó sóng âm được vạch hoặc rập trong đường rãnh xoắn ốc liên tục."@vi ,
                                                                                                                          "Objeto con forma de rollo en el cual se han hecho incisiones o muescas en un surco circular continuo."@es ,
                                                                                                                          "Rullamuotoinen tallennetyyppi, johon ääniaallot on kaiverrettu tai uurrettu yhtenäisenä pyöreänä urana."@fi ,
                                                                                                                          "Tipus de suport físic que consisteix en un objecte en forma de rotlle en el qual s’han gravat ones sonores per mitjà d’incisions o marques tot creant un solc circular continu."@ca ,
                                                                                                                          "Type de support matériel qui consiste en un objet en forme de rouleau sur lequel des ondulations sonores ont été gravées au moyen d’une entaille ou d’empreintes en créant un sillon circulaire continu."@fr ,
                                                                                                                          "通过刻痕或连续的螺旋式纹槽在其上记录声波的滚筒形物体，包括蜡滚筒、金属丝滚筒等。"@zh ;
                                                       <http://metadataregistry.org/uri/profile/rdakit/toolkitLabel> "Phonographenzylinder"@de ,
                                                                                                                     "audio cylinder"@en ,
                                                                                                                     "audiocilinder"@nl ,
                                                                                                                     "cilindre àudio"@ca ,
                                                                                                                     "cilindro audio"@it ,
                                                                                                                     "cilindro sonoro"@es ,
                                                                                                                     "cylindre audio"@fr ,
                                                                                                                     "fonografrull"@no ,
                                                                                                                     "ljudcylinder"@sv ,
                                                                                                                     "lydvalse"@da ,
                                                                                                                     "trục lăn audio"@vi ,
                                                                                                                     "äänisylinteri"@fi ,
                                                                                                                     "录音筒"@zh ;
                                                       <http://metadataregistry.org/uri/profile/regap/identifier> <http://metadataregistry.org/concepts/535> ;
                                                       rdfs:label "audio cylinder" ;
                                                       <http://www.w3.org/2004/02/skos/core#definition> "A carrier type consisting of a roller-shaped object on which sound waves are incised or indented in a continuous circular groove."@en ,
                                                                                                        "Bærertype, der består af et rulleformet genstand, hvorpå lydbølger er indskåret eller indtrykt i en uafbrudt cirkulær rille."@da ,
                                                                                                        "Een rolvormig object waarop geluidsgolven worden ingesneden of ingesprongen in een continue cirkelvormige groef."@nl ,
                                                                                                        "Ein Datenträgertyp, der aus einem rollenförmigen Objekt besteht, auf dem Schallwellen in einer fortlaufend gewundenen Rille graviert oder eingeprägt sind."@de ,
                                                                                                        "En bærertype som består av en sylinderformet gjenstand der lydopptak er gravert inn i et uavbrutt, sirkulært spor."@no ,
                                                                                                        "Loại hộp chứa gồm có vật thể hình trục lăn trên đó sóng âm được vạch hoặc rập trong đường rãnh xoắn ốc liên tục."@vi ,
                                                                                                        "Objeto con forma de rollo en el cual se han hecho incisiones o muescas en un surco circular continuo."@es ,
                                                                                                        "Rullamuotoinen tallennetyyppi, johon ääniaallot on kaiverrettu tai uurrettu yhtenäisenä pyöreänä urana."@fi ,
                                                                                                        "Tipus de suport físic que consisteix en un objecte en forma de rotlle en el qual s’han gravat ones sonores per mitjà d’incisions o marques tot creant un solc circular continu."@ca ,
                                                                                                        "Type de support matériel qui consiste en un objet en forme de rouleau sur lequel des ondulations sonores ont été gravées au moyen d’une entaille ou d’empreintes en créant un sillon circulaire continu."@fr ,
                                                                                                        "通过刻痕或连续的螺旋式纹槽在其上记录声波的滚筒形物体，包括蜡滚筒、金属丝滚筒等。"@zh ;
                                                       <http://www.w3.org/2004/02/skos/core#inScheme> <http://rdaregistry.info/termList/RDACarrierType> ;
                                                       <http://www.w3.org/2004/02/skos/core#prefLabel> "Phonographenzylinder"@de ,
                                                                                                       "audio cylinder"@en ,
                                                                                                       "audiocilinder"@nl ,
                                                                                                       "cilindre àudio"@ca ,
                                                                                                       "cilindro audio"@it ,
                                                                                                       "cilindro sonoro"@es ,
                                                                                                       "cylindre audio"@fr ,
                                                                                                       "fonografrull"@no ,
                                                                                                       "ljudcylinder"@sv ,
                                                                                                       "lydvalse"@da ,
                                                                                                       "trục lăn audio"@vi ,
                                                                                                       "äänisylinteri"@fi ,
                                                                                                       "أسطوانة سمعية"@ar ,
                                                                                                       "录音筒"@zh ;
                                                       <http://www.w3.org/2004/02/skos/core#scopeNote> "Comprend les cylindres de cire, cylindres de fil, etc."@fr ,
                                                                                                       "Dazu gehören Wachszylinder, Drahtzylinder usw."@de ,
                                                                                                       "Esim. vahasylinteri, vaijerisylinteri."@fi ,
                                                                                                       "Inclou cilindres de cera, de filferro, etc."@ca ,
                                                                                                       "Incluye cilindros de cera, cilindros metálicos, etc."@es ,
                                                                                                       "Trục lăn sáp, trục lăn dây, v.v..., được bao gồm"@vi ,
                                                                                                       "Vokssylindre, sylindre med metalltråd, etc. er inkludert."@no ,
                                                                                                       "Wax cylinders, wire cylinders, etc., are included."@en ,
                                                                                                       "包括腊筒、线筒等"@zh .


###  http://rdaregistry.info/termList/RDACarrierType/1004
<http://rdaregistry.info/termList/RDACarrierType/1004> rdf:type owl:NamedIndividual ,
                                                                <http://www.w3.org/2004/02/skos/core#Concept> ;
                                                       <http://metadataregistry.org/uri/profile/rdakit/toolkitDefinition> "A carrier type consisting of a disc on which sound waves, recorded as modulations, pulses, etc., are incised or indented in a continuous spiral groove."@en ,
                                                                                                                          "Bærertype, der består af en disc eller plade, hvorpå lydbølger optaget som modulationer, rytmer etc. er ridset eller indtrykt i en uafbrudt cirkulær rille."@da ,
                                                                                                                          "Disco en el que las ondas sonoras, registradas como modulaciones, pulsos, etc., se registraron mediante incisiones o muescas en un surco en espiral continua."@es ,
                                                                                                                          "Een disc waarop geluidsgolven, opgeslagen als modulaties, pulsen etc., ingesneden of ingesprongen zijn in een continue spiraalvormige groef."@nl ,
                                                                                                                          "Ein Datenträgertyp, der aus einer Disk besteht, auf der als Modulation, Pulse usw. aufgenommene Schallwellen in einer fortlaufend gewundenen Rille graviert oder eingeprägt sind."@de ,
                                                                                                                          "En bærertype som består av en plate der lydbølger, registrert som modulasjoner, pulser, etc. er gravert inn i et uavbrutt, spiralformet spor."@no ,
                                                                                                                          "Levy, jolle on kaiverrettu tai uurrettu modulaatioiksi tai pulsseiksi tallennettuja äänisignaaleja yhtenäiseksi spiraalimaiseksi uraksi."@fi ,
                                                                                                                          "Loại hộp chứa gồm có đĩa trên đó sóng âm ghi lại như là chuyển giọng, nhịp điệu, vv... được vạch hoặc rập trong đường rãnh xoắn ốc liên tục."@vi ,
                                                                                                                          "Tipus de suport físic que consisteix en un disc en el qual s’han gravat ones sonores, enregistrades com a modulacions, impulsos, etc., per mitjà d’incisions o marques en un solc continu en espiral."@ca ,
                                                                                                                          "Type de support matériel qui consiste en un disque sur lequel des ondulations sonores, enregistrées sous forme de modulations, d’impulsions, etc., ont été gravées au moyen d’une entaille ou d’empreintes en créant un sillon continu en spirale."@fr ,
                                                                                                                          "通过刻痕或连续的螺旋式纹槽在其上将声波记录为音调、节奏等的盘片。"@zh ;
                                                       <http://metadataregistry.org/uri/profile/rdakit/toolkitLabel> "Audiodisk"@de ,
                                                                                                                     "audio disc"@en ,
                                                                                                                     "audiodisc"@nl ,
                                                                                                                     "disc àudio"@ca ,
                                                                                                                     "disco audio"@it ,
                                                                                                                     "disco sonoro"@es ,
                                                                                                                     "disque audio"@fr ,
                                                                                                                     "grammofonplate"@no ,
                                                                                                                     "ljudskiva"@sv ,
                                                                                                                     "lyddisc"@da ,
                                                                                                                     "äänilevy"@fi ,
                                                                                                                     "đĩa audio"@vi ,
                                                                                                                     "录音盘"@zh ;
                                                       <http://metadataregistry.org/uri/profile/regap/identifier> <http://metadataregistry.org/concepts/536> ;
                                                       rdfs:label "audio disc" ;
                                                       <http://www.w3.org/2004/02/skos/core#altLabel> "audiodisc"@da ,
                                                                                                      "disc sonor"@ca ,
                                                                                                      "disco de audio"@es ,
                                                                                                      "disque sonore"@fr ,
                                                                                                      "sound disc"@en ,
                                                                                                      "đĩa âm thanh"@vi ,
                                                                                                      "声音盘"@zh ;
                                                       <http://www.w3.org/2004/02/skos/core#definition> "A carrier type consisting of a disc on which sound waves, recorded as modulations, pulses, etc., are incised or indented in a continuous spiral groove."@en ,
                                                                                                        "Bærertype, der består af en disc eller plade, hvorpå lydbølger optaget som modulationer, rytmer etc. er ridset eller indtrykt i en uafbrudt cirkulær rille."@da ,
                                                                                                        "Disco en el que las ondas sonoras, registradas como modulaciones, pulsos, etc., se registraron mediante incisiones o muescas en un surco en espiral continua."@es ,
                                                                                                        "Een disc waarop geluidsgolven, opgeslagen als modulaties, pulsen etc., ingesneden of ingesprongen zijn in een continue spiraalvormige groef."@nl ,
                                                                                                        "Ein Datenträgertyp, der aus einer Disk besteht, auf der als Modulation, Pulse usw. aufgenommene Schallwellen in einer fortlaufend gewundenen Rille graviert oder eingeprägt sind."@de ,
                                                                                                        "En bærertype som består av en plate der lydbølger, registrert som modulasjoner, pulser, etc. er gravert inn i et uavbrutt, spiralformet spor."@no ,
                                                                                                        "Levy, jolle on kaiverrettu tai uurrettu modulaatioiksi tai pulsseiksi tallennettuja äänisignaaleja yhtenäiseksi spiraalimaiseksi uraksi."@fi ,
                                                                                                        "Loại hộp chứa gồm có đĩa trên đó sóng âm ghi lại như là chuyển giọng, nhịp điệu, vv... được vạch hoặc rập trong đường rãnh xoắn ốc liên tục."@vi ,
                                                                                                        "Tipus de suport físic que consisteix en un disc en el qual s’han gravat ones sonores, enregistrades com a modulacions, impulsos, etc., per mitjà d’incisions o marques en un solc continu en espiral."@ca ,
                                                                                                        "Type de support matériel qui consiste en un disque sur lequel des ondulations sonores, enregistrées sous forme de modulations, d’impulsions, etc., ont été gravées au moyen d’une entaille ou d’empreintes en créant un sillon continu en spirale."@fr ,
                                                                                                        "通过刻痕或连续的螺旋式纹槽在其上将声波记录为音调、节奏等的盘片。"@zh ;
                                                       <http://www.w3.org/2004/02/skos/core#inScheme> <http://rdaregistry.info/termList/RDACarrierType> ;
                                                       <http://www.w3.org/2004/02/skos/core#narrower> :CdAudio ,
                                                                                                      :DvdAudio ,
                                                                                                      :EnhancedCdAudio ,
                                                                                                      :EpRecord ,
                                                                                                      :HybridSacd ,
                                                                                                      :Sacd ;
                                                       <http://www.w3.org/2004/02/skos/core#prefLabel> "Audiodisk"@de ,
                                                                                                       "audio disc"@en ,
                                                                                                       "audiodisc"@nl ,
                                                                                                       "disc àudio"@ca ,
                                                                                                       "disco audio"@it ,
                                                                                                       "disco sonoro"@es ,
                                                                                                       "disque audio"@fr ,
                                                                                                       "grammofonplate"@no ,
                                                                                                       "ljudskiva"@sv ,
                                                                                                       "lyddisc"@da ,
                                                                                                       "äänilevy"@fi ,
                                                                                                       "đĩa audio"@vi ,
                                                                                                       "قرص صوتي"@ar ,
                                                                                                       "录音盘"@zh .


###  http://rdaregistry.info/termList/RDACarrierType/1006
<http://rdaregistry.info/termList/RDACarrierType/1006> rdf:type owl:NamedIndividual ,
                                                                <http://www.w3.org/2004/02/skos/core#Concept> ;
                                                       <http://metadataregistry.org/uri/profile/rdakit/toolkitDefinition> "A carrier type consisting of a roll of paper on which musical notes are represented by perforations, designed to mechanically reproduce the music when used in a player piano, player organ, etc."@en ,
                                                                                                                          "Bærertype, der består af en papirrulle, hvorpå musiknoder repræsenteres af huller skabt til at gengive musikken mekanisk, når rullen bruges i et pianola, mekanisk klaver etc."@da ,
                                                                                                                          "Een rol papier waarop muzieknoten voorgesteld worden door perforaties, ontworpen om mechanisch de muziek weer te geven wanneer deze gebruikt wordt in een pianola e.d."@nl ,
                                                                                                                          "Ein Datenträgertyp, der aus einer Papierrolle besteht, auf der Musiknoten in Form von Perforationen repräsentiert werden und die konzipiert ist, um Musik in einem mechanischen Klavier, einer mechanischen Orgel usw. wiederzugeben."@de ,
                                                                                                                          "En bærertype som består av en papirrull der musikknoter representeres av hull, utformet for å gjengi musikken mekanisk ved bruk i pianola og lignende mekaniske instrumenter."@no ,
                                                                                                                          "Loại hộp chứa gồm có cuốn giấy trên đó nốt nhạc được trình bày bởi các lỗ răng cưa để tái tạo một cách cơ học âm nhạc khi dùng với piano tự động, organ tự động, vv..."@vi ,
                                                                                                                          "Paperirulla, jossa olevat rei’itykset edustavat toistettavia säveliä. Suunniteltu toistamaan musiikkia mekaanisesti automaattipianon, automaattiurkujen yms. avulla."@fi ,
                                                                                                                          "Rollo de papel en el que las notas musicales están representadas mediante perforaciones, diseñado para reproducir en forma mecánica la música cuando se utiliza en una pianola, órgano mecánico, etc."@es ,
                                                                                                                          "Tipus de suport físic que consisteix en un rotlle de paper sobre el qual es representen les notes musicals amb perforacions, concebut per reproduir la música mecànicament quan s’usa en una pianola, un orgue mecànic, etc."@ca ,
                                                                                                                          "Type de support matériel qui consiste en un rouleau de papier sur lequel les notes de musique sont représentées par des perforations, destiné à reproduire mécaniquement la musique lorsqu’il est utilisé avec un piano mécanique, un orgue mécanique, etc."@fr ,
                                                                                                                          "通过穿孔方式表示音符的纸卷，用于钢琴、风琴等时，以机械方式重现音乐。"@zh ;
                                                       <http://metadataregistry.org/uri/profile/rdakit/toolkitLabel> "Notenrolle"@de ,
                                                                                                                     "audio roll"@en ,
                                                                                                                     "audiorol"@nl ,
                                                                                                                     "cuốn audio"@vi ,
                                                                                                                     "ljudrulle"@sv ,
                                                                                                                     "lydrulle"@da ,
                                                                                                                     "pianorull"@no ,
                                                                                                                     "rollo sonoro"@es ,
                                                                                                                     "rotlle àudio"@ca ,
                                                                                                                     "rouleau audio"@fr ,
                                                                                                                     "rullo audio"@it ,
                                                                                                                     "äänirulla"@fi ,
                                                                                                                     "录音卷"@zh ;
                                                       <http://metadataregistry.org/uri/profile/regap/identifier> <http://metadataregistry.org/concepts/538> ;
                                                       rdfs:label "audio roll" ;
                                                       <http://www.w3.org/2004/02/skos/core#altLabel> "cuốn piano"@vi ,
                                                                                                      "piano roll"@en ,
                                                                                                      "pianolarulle"@da ,
                                                                                                      "pianorulla"@fi ,
                                                                                                      "rollo de piano"@es ,
                                                                                                      "rouleau pour piano"@fr ,
                                                                                                      "钢琴滚筒"@zh ;
                                                       <http://www.w3.org/2004/02/skos/core#definition> "A carrier type consisting of a roll of paper on which musical notes are represented by perforations, designed to mechanically reproduce the music when used in a player piano, player organ, etc."@en ,
                                                                                                        "Bærertype, der består af en papirrulle, hvorpå musiknoder repræsenteres af huller skabt til at gengive musikken mekanisk, når rullen bruges i et pianola, mekanisk klaver etc."@da ,
                                                                                                        "Een rol papier waarop muzieknoten voorgesteld worden door perforaties, ontworpen om mechanisch de muziek weer te geven wanneer deze gebruikt wordt in een pianola e.d."@nl ,
                                                                                                        "Ein Datenträgertyp, der aus einer Papierrolle besteht, auf der Musiknoten in Form von Perforationen repräsentiert werden und die konzipiert ist, um Musik in einem mechanischen Klavier, einer mechanischen Orgel usw. wiederzugeben."@de ,
                                                                                                        "En bærertype som består av en papirrull der musikknoter representeres av hull, utformet for å gjengi musikken mekanisk ved bruk i pianola og lignende mekaniske instrumenter."@no ,
                                                                                                        "Loại hộp chứa gồm có cuốn giấy trên đó nốt nhạc được trình bày bởi các lỗ răng cưa để tái tạo một cách cơ học âm nhạc khi dùng với piano tự động, organ tự động, vv..."@vi ,
                                                                                                        "Paperirulla, jossa olevat rei’itykset edustavat toistettavia säveliä. Suunniteltu toistamaan musiikkia mekaanisesti automaattipianon, automaattiurkujen yms. avulla."@fi ,
                                                                                                        "Rollo de papel en el que las notas musicales están representadas mediante perforaciones, diseñado para reproducir en forma mecánica la música cuando se utiliza en una pianola, órgano mecánico, etc."@es ,
                                                                                                        "Tipus de suport físic que consisteix en un rotlle de paper sobre el qual es representen les notes musicals amb perforacions, concebut per reproduir la música mecànicament quan s’usa en una pianola, un orgue mecànic, etc."@ca ,
                                                                                                        "Type de support matériel qui consiste en un rouleau de papier sur lequel les notes de musique sont représentées par des perforations, destiné à reproduire mécaniquement la musique lorsqu’il est utilisé avec un piano mécanique, un orgue mécanique, etc."@fr ,
                                                                                                        "通过穿孔方式表示音符的纸卷，用于钢琴、风琴等时，以机械方式重现音乐。"@zh ;
                                                       <http://www.w3.org/2004/02/skos/core#inScheme> <http://rdaregistry.info/termList/RDACarrierType> ;
                                                       <http://www.w3.org/2004/02/skos/core#narrower> :OrganRoll ,
                                                                                                      :PianoRoll ;
                                                       <http://www.w3.org/2004/02/skos/core#prefLabel> "Notenrolle"@de ,
                                                                                                       "audio roll"@en ,
                                                                                                       "audiorol"@nl ,
                                                                                                       "cuốn audio"@vi ,
                                                                                                       "ljudrulle"@sv ,
                                                                                                       "lydrulle"@da ,
                                                                                                       "pianorull"@no ,
                                                                                                       "rollo sonoro"@es ,
                                                                                                       "rotlle àudio"@ca ,
                                                                                                       "rouleau audio"@fr ,
                                                                                                       "rullo audio"@it ,
                                                                                                       "äänirulla"@fi ,
                                                                                                       "لفافة سمعية"@ar ,
                                                                                                       "录音卷"@zh ;
                                                       <http://www.w3.org/2004/02/skos/core#scopeNote> "Incluye rollos de pianola, etc."@es ,
                                                                                                       "用于钢琴滚筒等。"@zh .


###  http://rdaregistry.info/termList/RDACarrierType/1007
<http://rdaregistry.info/termList/RDACarrierType/1007> rdf:type owl:NamedIndividual ,
                                                                <http://www.w3.org/2004/02/skos/core#Concept> ;
                                                       <http://metadataregistry.org/uri/profile/rdakit/toolkitDefinition> "A carrier type consisting of a cassette containing an audiotape."@en ,
                                                                                                                          "Bærertype, der består af en kassette, der indeholder et lydbånd."@da ,
                                                                                                                          "Casete que contiene una cinta de audio."@es ,
                                                                                                                          "Een cassette die een audiotape bevat."@nl ,
                                                                                                                          "Ein Datenträgertyp, der aus einer Kassette besteht, die ein Tonband enthält."@de ,
                                                                                                                          "En bærertype som består av en kassett som inneholder et lydbånd."@no ,
                                                                                                                          "Kasetti, joka sisältää ääninauhan."@fi ,
                                                                                                                          "Loại hộp chứa gồm có cassette chứa một băng audio."@vi ,
                                                                                                                          "Tipus de suport físic que consisteix en una casset que conté una cinta àudio."@ca ,
                                                                                                                          "Type de support matériel qui consiste en une cassette contenant une bande audio."@fr ,
                                                                                                                          "装在双轴盒中的录音带。"@zh ;
                                                       <http://metadataregistry.org/uri/profile/rdakit/toolkitLabel> "Audiokassette"@de ,
                                                                                                                     "audiocasete"@es ,
                                                                                                                     "audiocassetta"@it ,
                                                                                                                     "audiocassette"@en ,
                                                                                                                     "audiocassette"@nl ,
                                                                                                                     "audiocassette"@vi ,
                                                                                                                     "casset àudio"@ca ,
                                                                                                                     "cassette audio"@fr ,
                                                                                                                     "kassettebånd"@da ,
                                                                                                                     "ljudkassett"@sv ,
                                                                                                                     "lydkassett"@no ,
                                                                                                                     "äänikasetti"@fi ,
                                                                                                                     "卡式录音带"@zh ;
                                                       <http://metadataregistry.org/uri/profile/regap/identifier> <http://metadataregistry.org/concepts/539> ;
                                                       rdfs:label "audiocassette" ;
                                                       <http://www.w3.org/2004/02/skos/core#definition> "A carrier type consisting of a cassette containing an audiotape."@en ,
                                                                                                        "Bærertype, der består af en kassette, der indeholder et lydbånd."@da ,
                                                                                                        "Casete que contiene una cinta de audio."@es ,
                                                                                                        "Een cassette die een audiotape bevat."@nl ,
                                                                                                        "Ein Datenträgertyp, der aus einer Kassette besteht, die ein Tonband enthält."@de ,
                                                                                                        "En bærertype som består av en kassett som inneholder et lydbånd."@no ,
                                                                                                        "Kasetti, joka sisältää ääninauhan."@fi ,
                                                                                                        "Loại hộp chứa gồm có cassette chứa một băng audio."@vi ,
                                                                                                        "Tipus de suport físic que consisteix en una casset que conté una cinta àudio."@ca ,
                                                                                                        "Type de support matériel qui consiste en une cassette contenant une bande audio."@fr ,
                                                                                                        "装在双轴盒中的录音带。"@zh ;
                                                       <http://www.w3.org/2004/02/skos/core#inScheme> <http://rdaregistry.info/termList/RDACarrierType> ;
                                                       <http://www.w3.org/2004/02/skos/core#narrower> :DAT ;
                                                       <http://www.w3.org/2004/02/skos/core#prefLabel> "Audiokassette"@de ,
                                                                                                       "audiocasete"@es ,
                                                                                                       "audiocassetta"@it ,
                                                                                                       "audiocassette"@en ,
                                                                                                       "audiocassette"@nl ,
                                                                                                       "audiocassette"@vi ,
                                                                                                       "casset àudio"@ca ,
                                                                                                       "cassette audio"@fr ,
                                                                                                       "kassettebånd"@da ,
                                                                                                       "ljudkassett"@sv ,
                                                                                                       "lydkassett"@no ,
                                                                                                       "äänikasetti"@fi ,
                                                                                                       "كاسيت صوتي"@ar ,
                                                                                                       "卡式录音带"@zh .


###  http://rdaregistry.info/termList/RDACarrierType/1060
<http://rdaregistry.info/termList/RDACarrierType/1060> rdf:type owl:NamedIndividual ,
                                                                <http://www.w3.org/2004/02/skos/core#Concept> ;
                                                       <http://metadataregistry.org/uri/profile/rdakit/toolkitDefinition> "A carrier type consisting of a disc on which video signals, with or without sound, are recorded."@en ,
                                                                                                                          "Bærertype, der består af en disc, hvorpå der er optaget videosignaler med eller uden lyd."@da ,
                                                                                                                          "Disco sobre el que se han grabado señales de video, con o sin sonido."@es ,
                                                                                                                          "Een disc waarop videosignalen, met of zonder geluid, worden opgenomen."@nl ,
                                                                                                                          "Ein Datenträgertyp, der aus eine Disk besteht, auf der Video-Signale mit oder ohne Ton aufgezeichnet sind."@de ,
                                                                                                                          "En bærertype som består av en plate der videosignaler med eller uten lyd registreres."@no ,
                                                                                                                          "Levy, jolle tallennetaan videosignaaleja, sisältäen ääntä tai ilman ääntä."@fi ,
                                                                                                                          "Loại hộp chứa gồm có đĩa trên đó tín hiệu video, có hoặc không có âm thanh, được ghi lại."@vi ,
                                                                                                                          "Tipus de suport físic que consisteix en un disc en el qual hi ha enregistrats senyals de vídeo, amb o sense so."@ca ,
                                                                                                                          "Type de support matériel qui consiste en un disque sur lequel des signaux vidéo, accompagnés ou non de son, sont enregistrés."@fr ,
                                                                                                                          "记录视频信号的盘片，有无声音均可。"@zh ;
                                                       <http://metadataregistry.org/uri/profile/rdakit/toolkitLabel> "Videodisk"@de ,
                                                                                                                     "videodisc"@ca ,
                                                                                                                     "videodisc"@da ,
                                                                                                                     "videodisc"@en ,
                                                                                                                     "videodisc"@nl ,
                                                                                                                     "videodisco"@es ,
                                                                                                                     "videodisco"@it ,
                                                                                                                     "videodisk"@no ,
                                                                                                                     "videolevy"@fi ,
                                                                                                                     "videoskiva"@sv ,
                                                                                                                     "vidéodisque"@fr ,
                                                                                                                     "đĩa video"@vi ,
                                                                                                                     "视盘"@zh ;
                                                       <http://metadataregistry.org/uri/profile/regap/identifier> <http://metadataregistry.org/concepts/1113> ;
                                                       rdfs:label "videodisc" ;
                                                       <http://www.w3.org/2004/02/skos/core#definition> "A carrier type consisting of a disc on which video signals, with or without sound, are recorded."@en ,
                                                                                                        "Bærertype, der består af en disc, hvorpå der er optaget videosignaler med eller uden lyd."@da ,
                                                                                                        "Disco sobre el que se han grabado señales de video, con o sin sonido."@es ,
                                                                                                        "Een disc waarop videosignalen, met of zonder geluid, worden opgenomen."@nl ,
                                                                                                        "Ein Datenträgertyp, der aus eine Disk besteht, auf der Video-Signale mit oder ohne Ton aufgezeichnet sind."@de ,
                                                                                                        "En bærertype som består av en plate der videosignaler med eller uten lyd registreres."@no ,
                                                                                                        "Levy, jolle tallennetaan videosignaaleja, sisältäen ääntä tai ilman ääntä."@fi ,
                                                                                                        "Loại hộp chứa gồm có đĩa trên đó tín hiệu video, có hoặc không có âm thanh, được ghi lại."@vi ,
                                                                                                        "Tipus de suport físic que consisteix en un disc en el qual hi ha enregistrats senyals de vídeo, amb o sense so."@ca ,
                                                                                                        "Type de support matériel qui consiste en un disque sur lequel des signaux vidéo, accompagnés ou non de son, sont enregistrés."@fr ,
                                                                                                        "记录视频信号的盘片，有无声音均可。"@zh ;
                                                       <http://www.w3.org/2004/02/skos/core#inScheme> <http://rdaregistry.info/termList/RDACarrierType> ;
                                                       <http://www.w3.org/2004/02/skos/core#narrower> :DvdVideo ;
                                                       <http://www.w3.org/2004/02/skos/core#prefLabel> "Videodisk"@de ,
                                                                                                       "videodisc"@ca ,
                                                                                                       "videodisc"@da ,
                                                                                                       "videodisc"@en ,
                                                                                                       "videodisc"@nl ,
                                                                                                       "videodisco"@es ,
                                                                                                       "videodisco"@it ,
                                                                                                       "videodisk"@no ,
                                                                                                       "videolevy"@fi ,
                                                                                                       "videoskiva"@sv ,
                                                                                                       "vidéodisque"@fr ,
                                                                                                       "đĩa video"@vi ,
                                                                                                       "قرص فيديو"@ar ,
                                                                                                       "视盘"@zh .


###  Generated by the OWL API (version 4.2.8.20170104-2310) https://github.com/owlcs/owlapi
